TermTests/DispatchAndFoldTest.lean
@@ -91,6 +91,12 @@ error: could not synthesize default value for parameter 'hRec' using tactics
 error: Tactic `decide` proved that the proposition
   0 < Usage.sumN (TyWf.prim LeanPrimTy.nat) (0 + 1) (Usage.single DeBruijn.head).tail
 is false
+---
+error: could not synthesize default value for parameter 'hStep' using tactics
+---
+error: Tactic `decide` proved that the proposition
+  0 = 0 → Head.var ≠ Head.var
+is false
 -/
 #guard_msgs (error) in
 def foldNoAnswer :=
@@ -117,7 +123,7 @@ info: ((Term.var DeBruijnProj.head.tail).bool_casesOn
         (fun vs => LeanInitPureExtern.preludeExtern (PreludeExtern.lean_nat_add vs.1 vs.2.1)) appIfDef_term._proof_4)
       (Term.externCall (Spine.cons (Term.var DeBruijnProj.head) (Spine.cons (Term.nat_mk 2) Spine.nil))
         (fun vs => LeanInitPureExtern.preludeExtern (PreludeExtern.lean_nat_mul vs.1 vs.2.1)) appIfDef_term._proof_4)
-      appIfDef_term._proof_5).lam.lam
+      appIfDef_term._proof_5 appIfDef_term._proof_6).lam.lam
 -/
 #guard_msgs in
 #reduce (proofs := false) (types := false) appIfDef_term
@@ -141,8 +147,8 @@ info: ((Term.externCall (Spine.cons (Term.var DeBruijnProj.head) (Spine.cons (Te
         (Term.externCall (Spine.cons (Term.var DeBruijnProj.head) (Spine.cons (Term.var DeBruijnProj.head) Spine.nil))
           (fun vs => LeanInitPureExtern.preludeExtern (PreludeExtern.lean_nat_add vs.1 vs.2.1))
           appIfCompDef_term._proof_1)
-        (Term.nat_mk 0) appIfDef_term._proof_5)
-      appIfCompDef_term._proof_2 ⋯).lam.lam
+        (Term.nat_mk 0) appIfDef_term._proof_5 appIfCompDef_term._proof_2)
+      appIfCompDef_term._proof_3 ⋯).lam.lam
 -/
 #guard_msgs in
 #reduce (proofs := false) (types := false) appIfCompDef_term
@@ -157,7 +163,8 @@ def forceIfDef_term :=
 
 /--
 info: ((Term.var DeBruijnProj.head.tail).bool_casesOn (Term.nat_mk 5)
-      ((Term.var DeBruijnProj.head).thunk_force forceIfDef_term._proof_3) appIfDef_term._proof_5).lam.lam
+      ((Term.var DeBruijnProj.head).thunk_force forceIfDef_term._proof_3) appIfDef_term._proof_5
+      forceIfDef_term._proof_4).lam.lam
 -/
 #guard_msgs in
 #reduce (proofs := false) (types := false) forceIfDef_term
